ver2_qbft_Style/Lemmas.dfy
@@ -1,0 +1,15 @@
+include "Type.dfy"
+include "Auxilarily.dfy"
+
+module M_Lemma {
+    import opened M_SpecTypes
+    import opened M_AuxilarilyFunc
+
+    lemma LemmaViewDiffOnConflictCertificate(cert1 : Cert, cert2 : Cert)
+    requires ValidQC(cert1) && ValidQC(cert2)
+    requires !NoConflict(cert1.block, cert2.block)
+    ensures cert1.viewNum != cert2.viewNum
+    {
+
+    }
+}
